Let $f : A \rightarrow B$ and $g : B \rightarrow C$. If $f$ and $g$ are both one-to-one functions, show that $g \circ f$ is one-to-one

*Proof*

Let $f : A \rightarrow B$, f is one-to-one
&nbsp;

and $g : B \rightarrow C$, g is one to one

Suppose we have to elements $a_1, a_2 \in A$ and that $(g \circ f)(a_1) = (g \circ f)(a_2)$. We have

&emsp; $g(f(a_1)) = g(f(a_2))$

&emsp; $f(a_1) = f(a_2)$

&emsp; $a_1 = a_2$

Hence, $(g \circ f)(a_1) = (g \circ f)(a_2)$ implies $a_1 = a_2$ and $g \circ f$ is one-to-one